proved substitution lemma

isabelle/AbstractBindingTrees.thy
@@ -13,7 +13,7 @@ interpretation abt_s: substable "Var 0" "rename Suc" "Var" "\<lambda> x. x"
   apply (auto simp add: rename_def)
   done
  
-abbreviation exts :: "('op ABT) sub \<Rightarrow> ('op ABT) sub" where
+definition exts :: "('op ABT) sub \<Rightarrow> ('op ABT) sub" where
   "exts \<sigma> \<equiv> abt_s.ext \<sigma>"
 
 definition subst :: "('op ABT) sub \<Rightarrow> 'op ABT \<Rightarrow> 'op ABT" ("\<llangle>_\<rrangle>") where
@@ -21,13 +21,6 @@ definition subst :: "('op ABT) sub \<Rightarrow> 'op ABT \<Rightarrow> 'op ABT" 
 
 abbreviation ren_sub :: "var sub \<Rightarrow> ('op ABT) sub" ("\<lceil>_\<rceil>") where
   "\<lceil>\<rho>\<rceil> x \<equiv> Var (\<rho> x)"
-
-fun subst_zero :: "'op ABT \<Rightarrow> var \<Rightarrow> 'op ABT" where
-  "subst_zero M 0 = M" |
-  "subst_zero M (Suc x) = Var x"
-
-abbreviation subst_one :: "'op ABT \<Rightarrow> 'op ABT \<Rightarrow> 'op ABT" ("_[_]" 70) where
-  "subst_one N M \<equiv> \<llangle> subst_zero M \<rrangle> N"
 
 definition seqss :: "('op ABT) sub \<Rightarrow> ('op ABT) sub \<Rightarrow> ('op ABT) sub" (infixr ";" 70) where
   "(\<sigma> ; \<tau>) x \<equiv> \<llangle>\<tau>\<rrangle> (\<sigma> x)"
@@ -38,20 +31,24 @@ definition seqrs :: "var sub \<Rightarrow> ('op ABT) sub \<Rightarrow> ('op ABT)
 definition seqsr :: "('op ABT) sub \<Rightarrow> var sub \<Rightarrow> ('op ABT) sub" (infixr ";r" 70) where
   "(\<sigma> ;r \<rho>) x \<equiv> rename \<rho> (\<sigma> x)"
 
-definition id :: "('op ABT) sub" where
-  "id x \<equiv> Var x"
+definition \<iota> :: "('op ABT) sub" where
+  "\<iota> x \<equiv> Var x"
+
+definition subst_one :: "'op ABT \<Rightarrow> 'op ABT \<Rightarrow> 'op ABT" ("_[_]" 70) where
+  "subst_one N M \<equiv> \<llangle> M \<bullet> \<iota> \<rrangle> N"
+declare subst_one_def[simp]
 
 lemma lift_seq_suc: "abt_s.lift_sub \<sigma> = \<sigma> ;r Suc"
   unfolding seqsr_def by simp
 
-theorem IdL[simp]: "id ; \<sigma> = \<sigma>"
-  unfolding subst_def id_def seqss_def by simp
+theorem IdL[simp]: "\<iota> ; \<sigma> = \<sigma>"
+  unfolding subst_def \<iota>_def seqss_def by simp
 
-theorem ShiftId[simp]:  "(\<up> ; id) = \<up>"
-  unfolding subst_def seqss_def id_def shift_def by simp
+theorem ShiftId[simp]:  "(\<up> ; \<iota>) = \<up>"
+  unfolding subst_def seqss_def \<iota>_def shift_def by simp
 
-theorem VarId[simp]: "\<llangle>id\<rrangle> (Var x) = Var x"
-  unfolding subst_def id_def by simp
+theorem VarId[simp]: "\<llangle>\<iota>\<rrangle> (Var x) = Var x"
+  unfolding subst_def \<iota>_def by simp
 
 theorem HeadCons[simp]: "(M \<bullet> \<sigma>) 0 = M"
   unfolding cons_def subst_def by simp
@@ -71,10 +68,10 @@ theorem ShiftCons[simp]: "\<up> ; (M \<bullet> \<sigma>) = \<sigma>"
 interpretation abt_sqs: subst_quote_shift "Var 0" "rename Suc" Var "\<lambda> x. x"
   by unfold_locales auto
 
-theorem subst_id[simp]: "\<llangle>id\<rrangle> M = M"
-  unfolding subst_def id_def by (rule abt_sqs.map_abt_id) simp
+theorem subst_id[simp]: "\<llangle>\<iota>\<rrangle> M = M"
+  unfolding subst_def \<iota>_def by (rule abt_sqs.map_abt_id) simp
   
-theorem IdR[simp]: "\<sigma> ; id = \<sigma>"
+theorem IdR[simp]: "\<sigma> ; \<iota> = \<sigma>"
   unfolding seqss_def by (rule ext) simp
 
 theorem ConsSeq[simp]: "(M \<bullet> \<sigma>) ; \<tau> = \<llangle> \<tau> \<rrangle> M \<bullet> (\<sigma> ; \<tau>)"
@@ -110,13 +107,13 @@ proof clarify
   show "\<lceil>extr \<sigma>\<rceil> x = (exts \<tau>) x" 
   proof (cases x)
     case 0
-    then show ?thesis by simp
+    then show ?thesis unfolding exts_def by simp
   next
     case (Suc y)
     with Suc have "\<lceil>extr \<sigma>\<rceil> x = Var (Suc (\<sigma> y))" by (simp add: cons_def seqrr_def)
     also have "... = rename Suc (Var (\<sigma> y))" unfolding rename_def by simp
     also have "... = rename Suc (\<tau> y)" using st by simp
-    also have "... = exts \<tau> x" using Suc by (simp add: cons_def)
+    also have "... = exts \<tau> x" using Suc unfolding exts_def by (simp add: cons_def)
     finally show ?thesis .
   qed  
 qed
@@ -125,7 +122,7 @@ theorem rename_subst: "rename \<rho> M = \<llangle> \<lceil> \<rho> \<rceil> \<r
 proof -
   have 1: "ren_sub.cong \<rho> \<lceil>\<rho>\<rceil>" by auto
   from 1 cong_ext have "var_s.map_abt \<rho> M = abt_s.map_abt \<lceil>\<rho>\<rceil> M" 
-    unfolding extr_def apply (rule ren_sub.map_cong) by simp
+    unfolding extr_def exts_def apply (rule ren_sub.map_cong) by simp
   then show ?thesis unfolding subst_def rename_def by auto
 qed
 
@@ -140,7 +137,7 @@ lemma exts_cons_seq: "exts \<sigma> = Var 0 \<bullet> (\<sigma> ; \<up>)"
 proof -
   have 1: "(\<lambda> x. rename Suc (\<sigma> x)) = (\<lambda> x. \<llangle> \<lceil> Suc \<rceil> \<rrangle> (\<sigma> x))"
     using rename_subst[of Suc] by auto
-  have "exts \<sigma> = Var 0 \<bullet> (\<lambda> x. \<llangle> \<lceil> Suc \<rceil> \<rrangle> (\<sigma> x))" using 1 by simp
+  have "exts \<sigma> = Var 0 \<bullet> (\<lambda> x. \<llangle> \<lceil> Suc \<rceil> \<rrangle> (\<sigma> x))" using 1 unfolding exts_def by simp
   also have "... = Var 0 \<bullet> (\<sigma> ; \<up>)" unfolding seqss_def by simp
   finally show "exts \<sigma> = Var 0 \<bullet> (\<sigma> ; \<up>)" .
 qed
@@ -180,27 +177,25 @@ proof -
     then have 1: "(extr \<sigma>) r; (exts \<tau>) = (exts \<rho>)"
       by (rule rss_comp_cong_ext) 
     have "rss.comp_cong (abt_s.ext \<tau>) (var_s.ext \<sigma>) (abt_s.ext \<rho>)"
-      apply auto apply (case_tac x) apply force apply (auto simp add: exts_cons_seq)
+      apply auto apply (case_tac x) apply force 
     proof -
       fix x
-      have "((extr \<sigma>) r; (exts \<tau>)) (Suc x) = (exts \<rho>) (Suc x)" using 1 by simp
-      then have "(\<sigma> r; \<tau> ; \<lceil>Suc\<rceil>) x = (\<rho> ; \<lceil>Suc\<rceil>) x" by (simp add: exts_cons_seq)
-      then show "(\<tau> ; \<lceil>Suc\<rceil>) (\<sigma> x) = (\<rho> ; \<lceil>Suc\<rceil>) x" unfolding seqrs_def by simp
+      have "(extr \<sigma> r; exts \<tau>) x = (exts \<rho>) x " using 1 by auto
+      then show "abt_s.ext \<tau> (var_s.ext \<sigma> x) = abt_s.ext \<rho> x"
+        unfolding extr_def exts_def seqrs_def .
     qed      
   }
   then have 3: "\<forall>\<sigma> \<tau> \<rho>. rss.comp_cong \<tau> \<sigma> \<rho> \<longrightarrow> rss.comp_cong (exts \<tau>) (var_s.ext \<sigma>) (exts \<rho>)"
-     by blast
+    unfolding exts_def by blast
   from 2 3 have "abt_s.map_abt \<sigma> (var_s.map_abt \<rho> M) = abt_s.map_abt \<tau> M"
-    by (rule rss.map_fusion)
+    unfolding exts_def by (rule rss.map_fusion)
   then show ?thesis unfolding subst_def rename_def by simp  
 qed
 
 theorem assoc_SRS[simp]: "(\<sigma> ;r \<rho>) ; \<tau> = \<sigma> ; (\<rho> r; \<tau>)"
   unfolding seqsr_def seqss_def seqrs_def apply (rule ext)
   apply (rule subst_rename_fusion)
-  unfolding seqrs_def apply simp
-  done
-
+  unfolding seqrs_def by simp
 
 interpretation srs: 
   substable3 "Var 0" 
@@ -217,19 +212,19 @@ lemma srs_comp_cong_ext: fixes x :: var
   shows "rename (extr \<rho>) (exts \<sigma> x) = exts \<tau> x"
 proof (cases x)
   case 0
-  then show ?thesis by simp 
+  then show ?thesis unfolding exts_def by simp 
 next
   case (Suc y)
   have            "((exts \<sigma>) ;r (extr \<rho>)) x 
-                 = rename (extr \<rho>) (rename Suc (\<sigma> y))" using Suc seqsr_def by auto
+                 = rename (extr \<rho>) (rename Suc (\<sigma> y))" using Suc seqsr_def unfolding exts_def by auto
   also have "... = rename (Suc r;r (extr \<rho>)) (\<sigma> y)" 
     by (rule rename_fusion[of "(extr \<rho>)" Suc "\<sigma> y"])
   also have "... = rename (\<rho> r;r Suc) (\<sigma> y)" by simp
   also have "... = rename Suc (rename \<rho> (\<sigma> y))" using rename_fusion[of Suc \<rho> "\<sigma> y"] by auto
   also have "... = rename Suc ((\<sigma> ;r \<rho>) y)" unfolding seqsr_def ..
   also have "... = rename Suc (\<tau> y)" using cc by simp
-  also have "... = exts \<tau> x" using Suc by (simp add: cons_def)
-  finally have "((exts \<sigma>) ;r (extr \<rho>)) x = exts \<tau> x" by simp
+  also have "... = exts \<tau> x" using Suc unfolding exts_def by (simp add: cons_def)
+  finally have "((exts \<sigma>) ;r (extr \<rho>)) x = exts \<tau> x" unfolding exts_def by simp
   then show ?thesis unfolding seqsr_def by simp
 qed
 
@@ -244,8 +239,8 @@ proof -
     fix \<sigma> \<tau> \<rho> x assume "srs.comp_cong \<tau> \<sigma> \<rho>"
     then have "\<sigma> ;r \<tau> = \<rho>" unfolding seqsr_def rename_def by auto
     then have "rename (extr \<tau>) (exts \<sigma> x) = exts \<rho> x" by (rule srs_comp_cong_ext)
-    then show "var_s.map_abt (var_s.ext \<tau>) (exts \<sigma> x) = exts \<rho> x"
-      unfolding rename_def extr_def by fast
+    then show "var_s.map_abt (var_s.ext \<tau>) (abt_s.ext \<sigma> x) = abt_s.ext \<rho> x"
+      unfolding rename_def extr_def exts_def by fast
   qed
   then show "rename \<rho> (\<llangle>\<sigma>\<rrangle> M) = \<llangle>\<sigma> ;r \<rho>\<rrangle> M"
     unfolding rename_def subst_def by fast
@@ -269,13 +264,11 @@ interpretation sss:
    "rename Suc" "\<lambda> x. x" Var
   by unfold_locales
 
-(*
-
 lemma ssscc_eq_seqss: "(\<sigma> ; \<rho> = \<tau>) = (sss.comp_cong \<rho> \<sigma> \<tau>)"
-  unfolding subst_def by auto
+  unfolding subst_def seqss_def by auto
 
 lemma seqss_eq_ssscc: "(sss.comp_cong \<rho> \<sigma> \<tau>) = (\<sigma> ; \<rho> = \<tau>)"
-  unfolding subst_def by auto
+  unfolding subst_def seqss_def by auto
 
 lemma sss_comp_cong_ext:
   fixes x :: var
@@ -283,46 +276,81 @@ lemma sss_comp_cong_ext:
   shows "((exts \<sigma>) ; (exts \<rho>)) x = exts \<tau> x"
 proof (cases x)
   case 0
-  then show ?thesis by (simp add: cons_def subst_def)
+  then show ?thesis unfolding exts_def by (simp add: subst_def)
 next
   case (Suc y)
-  have "(exts \<sigma> ; exts \<rho>) x = ((\<sigma> ;r Suc) ; (exts \<rho>)) y" using Suc by (simp add: cons_def)
-  also have "... = \<llangle>Suc r; exts \<rho>\<rrangle> (\<sigma> y)" using subst_rename_fusion[of "exts \<rho>" Suc "Suc r; exts \<rho>"] by auto
-  also have "... = rename Suc (\<llangle>\<rho>\<rrangle> (\<sigma> y))" 
-    using rename_subst_fusion[of Suc \<rho> "Suc r; exts \<rho>" "\<sigma> y"] by (auto simp add: cons_def)
-  also have "... = rename Suc (\<tau> y)" using 1 unfolding subst_def by auto
-  also have "... = exts \<tau> x" using Suc by (simp add: cons_def)
+  thm subst_rename_fusion
+  have "(exts \<sigma> ; exts \<rho>) x = \<llangle>exts \<rho>\<rrangle> (exts \<sigma> x)" unfolding seqss_def by simp
+  also have "... = \<llangle>exts \<rho>\<rrangle> (rename Suc (\<sigma> y))" using Suc unfolding exts_def by simp
+  also have "... = \<llangle>Suc r; exts \<rho>\<rrangle> (\<sigma> y)" by (rule subst_rename_fusion) simp
+  also have "... = \<llangle> \<rho> ;r Suc \<rrangle> (\<sigma> y)" unfolding seqsr_def seqrs_def exts_def by simp  
+  also have "... = rename Suc (\<llangle>\<rho>\<rrangle> (\<sigma> y))" using rename_subst_fusion[of Suc \<rho> "\<sigma> y"] by simp
+  also have "... = rename Suc (\<tau> y)" using 1 unfolding seqss_def by auto
+  also have "... = exts \<tau> x" using Suc unfolding exts_def by (simp add: cons_def)
   finally show ?thesis .
 qed
 
 theorem subst_subst_fusion: "\<llangle>\<rho>\<rrangle> (\<llangle>\<sigma>\<rrangle> M) = \<llangle>\<sigma> ; \<rho>\<rrangle> M"
-  unfolding subst_def apply (rule sss.map_fusion)
-   apply force
-proof clarify
-  fix \<sigma> \<tau> \<rho> x
-  assume 1: "sss.comp_cong \<tau> \<sigma> \<rho>" 
-  from 1 have "\<sigma> ; \<tau> = \<rho>" unfolding subst_def by auto
-  then have "(exts \<sigma> ; exts \<tau>) x = exts \<rho> x" by (rule sss_comp_cong_ext)
-  then show "abt_s.map_abt (exts \<tau>) (exts \<sigma> x) = exts \<rho> x" unfolding subst_def by simp
+proof -
+  have 1: "sss.comp_cong \<rho> \<sigma> (\<sigma> ; \<rho>)" unfolding seqss_def subst_def by auto
+  from 1 have "abt_s.map_abt \<rho> (abt_s.map_abt \<sigma> M) = abt_s.map_abt (\<sigma> ; \<rho>) M"
+  proof (rule sss.map_fusion, clarify)
+    fix \<sigma> \<tau> \<rho> x assume "sss.comp_cong \<tau> \<sigma> \<rho>"
+    then have "\<sigma> ; \<tau> = \<rho>" using seqss_eq_ssscc[of \<tau> \<sigma> \<rho>] by simp
+    then have "((exts \<sigma>) ; (exts \<tau>)) x = exts \<rho> x" by (rule sss_comp_cong_ext)
+    then show "abt_s.map_abt (abt_s.ext \<tau>) (abt_s.ext \<sigma> x) = abt_s.ext \<rho> x" 
+      unfolding seqss_def subst_def exts_def by simp
+  qed
+  then show ?thesis unfolding subst_def by simp
 qed
 
+declare subst_subst_fusion[simp]
 
-section "Lambda Calculus"
+theorem assoc_SSS[simp]: "(\<sigma> ; \<tau>) ; \<rho> = \<sigma> ; (\<tau> ; \<rho>)"
+proof (rule ext)
+  fix x
+  have "((\<sigma> ; \<tau>) ; \<rho>) x = \<llangle>\<rho>\<rrangle> (\<llangle>\<tau>\<rrangle> (\<sigma> x))" unfolding seqss_def by fast
+  also have "... = \<llangle> \<tau> ; \<rho> \<rrangle> (\<sigma> x)" by simp
+  also have "... = (\<sigma> ; (\<tau> ; \<rho>)) x" unfolding seqss_def by fast
+  finally show "((\<sigma> ; \<tau>) ; \<rho>) x = (\<sigma> ; \<tau> ; \<rho>) x" .
+qed
 
-datatype op_lam =
-  LamOp | AppOp
+declare exts_cons_seq[simp]
 
-type_synonym Term = "op_lam ABT"
+theorem subst_commute: "(\<llangle> exts \<sigma>\<rrangle> N) [ \<llangle> \<sigma> \<rrangle> M ] = \<llangle> \<sigma> \<rrangle> (N [ M ])"
+  by simp
 
-abbreviation Lam :: "Term \<Rightarrow> Term" ("\<lambda>") where 
-  "\<lambda> N \<equiv> App LamOp [Bnd (Trm N)]"
+theorem commute_subst: " \<llangle> \<sigma> \<rrangle> (N [ M ]) = (\<llangle> exts \<sigma>\<rrangle> N) [ \<llangle> \<sigma> \<rrangle> M ]"
+  using subst_commute by simp
 
-abbreviation Apply :: "Term \<Rightarrow> Term \<Rightarrow> Term" (infixl "\<cdot>" 60) where
-  "L \<cdot> M \<equiv> App AppOp [Trm L, Trm M]"
 
-inductive reduce :: "Term \<Rightarrow> Term \<Rightarrow> bool" (infix "\<longmapsto>" 50) where
-  beta: "(\<lambda> N) \<cdot> M \<longmapsto> N[M]"
-*)
+lemma rename_subst_cons[simp]: "\<lceil>y \<bullet> \<rho>\<rceil> = Var y \<bullet> \<lceil>\<rho>\<rceil>"
+  apply (rule ext) 
+  apply (case_tac x)
+   apply simp
+  apply simp
+  done
 
+lemma rename_subst_seq[simp]: "\<lceil>\<rho> r;r \<sigma>\<rceil> = \<lceil>\<rho>\<rceil> ; \<lceil>\<sigma>\<rceil>"
+proof (rule ext)
+  fix x
+  have "\<lceil>\<rho> r;r \<sigma>\<rceil> x = Var (\<sigma> (\<rho> x))" unfolding seqrr_def by simp
+  also have "... = \<llangle>\<lceil>\<sigma>\<rceil>\<rrangle> (Var (\<rho> x))" unfolding subst_def by simp
+  also have "... = \<llangle>\<lceil>\<sigma>\<rceil>\<rrangle> (\<lceil>\<rho>\<rceil> x)" by simp
+  also have "... = (\<lceil>\<rho>\<rceil> ; \<lceil>\<sigma>\<rceil>) x" unfolding seqss_def by simp
+  finally show "\<lceil>\<rho> r;r \<sigma>\<rceil> x = (\<lceil>\<rho>\<rceil> ; \<lceil>\<sigma>\<rceil>) x" .
+qed
+
+declare rename_subst[simp]
+
+theorem rename_subst_commute: "(rename (extr \<rho>) N) [ rename \<rho> M ] = rename \<rho> (N[M])"
+  by simp 
+
+definition subst_two :: "'op ABT \<Rightarrow> 'op ABT \<Rightarrow> 'op ABT" ("_\<lbrace>_\<rbrace>" 60) where
+ "N \<lbrace> M \<rbrace> = \<llangle> exts (M \<bullet> \<iota>) \<rrangle> N"
+declare subst_two_def[simp]
+
+theorem substitution: "M[N][L] = M\<lbrace>L\<rbrace>[N[L]]"
+  by simp
 
 end
