isabelle/LambdaExample.thy
@@ -1,0 +1,22 @@
+theory LambdaExample
+ imports Main AbstractBindingTrees
+begin
+
+section "Lambda Calculus"
+
+datatype op_lam =
+  LamOp | AppOp
+
+type_synonym Term = "op_lam ABT"
+
+abbreviation Lam :: "Term \<Rightarrow> Term" ("\<lambda>") where 
+  "\<lambda> N \<equiv> App LamOp [Bnd (Trm N)]"
+
+abbreviation Apply :: "Term \<Rightarrow> Term \<Rightarrow> Term" (infixl "\<cdot>" 60) where
+  "L \<cdot> M \<equiv> App AppOp [Trm L, Trm M]"
+
+inductive reduce :: "Term \<Rightarrow> Term \<Rightarrow> bool" (infix "\<longmapsto>" 50) where
+  beta: "(\<lambda> N) \<cdot> M \<longmapsto> N[M]"
+
+
+end
